add map_T_cong

scratch/Scratch.thy
@@ -13,19 +13,19 @@ term 0 (**)
 
 
 definition ceq :: "('a \<Rightarrow> 'a \<Rightarrow> bool) \<Rightarrow> ('param \<rightharpoonup> 'result, 'a) state \<Rightarrow> ('param \<rightharpoonup> 'result, 'a) state \<Rightarrow> bool" where
-  "ceq R s0 s1 \<equiv> (eq_onp consistentM ===> rel_prod R (eq_onp consistentM)) (runState s0) (runState s1)"
+  "ceq R s0 s1 \<equiv> (eq_onp cmem ===> rel_prod R (eq_onp cmem)) (runState s0) (runState s1)"
   
 lemma ceq_intro:
   fixes R s0 s1
-  assumes "\<And>M v0 M0 v1 M1. \<lbrakk>consistentM M; runState s0 M = (v0,M0); runState s1 M = (v1,M1)\<rbrakk> \<Longrightarrow> R v0 v1 \<and> M0=M1 \<and> consistentM M1"
+  assumes "\<And>M v0 M0 v1 M1. \<lbrakk>cmem M; runState s0 M = (v0,M0); runState s1 M = (v1,M1)\<rbrakk> \<Longrightarrow> R v0 v1 \<and> M0=M1 \<and> cmem M1"
   shows "ceq R s0 s1"
   unfolding ceq_def eq_onp_def rel_fun_def rel_prod_conv by (auto split: prod.split dest: assms)
 term 0 (**)
 
 lemma ceq_elim:
   fixes R s0 s1
-  assumes "ceq R s0 s1" "consistentM M"
-  obtains v0 M0 v1 M1 where "runState s0 M = (v0, M0)" "runState s1 M = (v1, M1)" "R v0 v1" "M0=M1" "consistentM M1"
+  assumes "ceq R s0 s1" "cmem M"
+  obtains v0 M0 v1 M1 where "runState s0 M = (v0, M0)" "runState s1 M = (v1, M1)" "R v0 v1" "M0=M1" "cmem M1"
   using assms unfolding ceq_def eq_onp_def rel_fun_def by (blast elim: rel_prod.cases)
     
 term 0 (**)
@@ -52,12 +52,17 @@ term 0 (**)
   
 lemma map\<^sub>T_cong:
   assumes "ceq R0 xs\<^sub>T ys\<^sub>T"
-  assumes "\<And>M. consistentM M \<Longrightarrow> case (runState f\<^sub>T M, runState g\<^sub>T M) of ((f, Mf), (g, Mg)) \<Rightarrow>
-            Mf = Mg \<and> consistentM Mg \<and> (case runState ys\<^sub>T Mg of (ys, Mys) \<Rightarrow> (\<forall>x\<in>set ys. ceq R1 (f x) (g x)))"
+  assumes "\<And>M. cmem M \<Longrightarrow> case (runState f\<^sub>T M, runState g\<^sub>T M) of ((f, Mf), (g, Mg)) \<Rightarrow>
+            Mf = Mg \<and> cmem Mg \<and> (case runState ys\<^sub>T Mg of (ys, Mys) \<Rightarrow> (\<forall>x\<in>set ys. ceq R1 (f x) (g x)))"
   shows "ceq (list_all2 R1) (map\<^sub>T . f\<^sub>T . xs\<^sub>T) (map\<^sub>T . g\<^sub>T . ys\<^sub>T)"
-
-
-
+  oops
+    
+lemma
+  assumes "ceq R0 xs\<^sub>T ys\<^sub>T"
+  assumes "\<And>M. cmem M \<Longrightarrow> case (runState f\<^sub>T M, runState g\<^sub>T M) of ((f, Mf), (g, Mg)) \<Rightarrow>
+            Mf = Mg \<and> cmem Mg \<and> (case runState ys\<^sub>T Mg of (ys, Mys) \<Rightarrow> (\<forall>x\<in>set ys. ceq R1 (f x) (g x)))"
+  assumes "ceq (\<lambda>f g. (\<forall>M. cmem M \<longrightarrow> )) f\<^sub>T g\<^sub>T"
+  shows "ceq (list_all2 R1) (map\<^sub>T . f\<^sub>T . xs\<^sub>T) (map\<^sub>T . g\<^sub>T . ys\<^sub>T)"
 
 
 
