DP_CRelSS.thy
@@ -1,0 +1,116 @@
+theory DP_CRelSS
+  imports "./DP_CRelVS" "./DP_CPredS"
+begin
+term int
+term fold
+  
+context dp_consistency
+begin
+context
+  includes lifting_syntax
+begin
+term 0 (**)
+
+
+definition crel_ss :: "('a \<Rightarrow> 'b \<Rightarrow> bool) \<Rightarrow> ('param \<rightharpoonup> 'result, 'a) state \<Rightarrow> ('param \<rightharpoonup> 'result, 'b) state \<Rightarrow> bool" where
+  "crel_ss R s0 s1 \<equiv> (eq_onp cmem ===> rel_prod R (eq_onp cmem)) (runState s0) (runState s1)"
+  
+lemma crel_ss_intro:
+  fixes R s0 s1
+  assumes "\<And>M v0 M0 v1 M1. \<lbrakk>cmem M; runState s0 M = (v0,M0); runState s1 M = (v1,M1)\<rbrakk> \<Longrightarrow> R v0 v1 \<and> M0=M1 \<and> cmem M1"
+  shows "crel_ss R s0 s1"
+  unfolding crel_ss_def eq_onp_def rel_fun_def rel_prod_conv by (auto split: prod.split dest: assms)
+term 0 (**)
+
+lemma crel_ss_elim:
+  fixes R s0 s1
+  assumes "crel_ss R s0 s1" "cmem M"
+  obtains v0 M0 v1 M1 where "runState s0 M = (v0, M0)" "runState s1 M = (v1, M1)" "R v0 v1" "M0=M1" "cmem M1"
+  using assms unfolding crel_ss_def eq_onp_def rel_fun_def by (blast elim: rel_prod.cases)
+    
+term 0 (**)
+  
+lemma id\<^sub>T_cong[transfer_rule]:
+  fixes R x y
+  shows "(R ===> crel_ss R) return return"
+  unfolding rel_fun_def return_def by (fastforce intro: crel_ss_intro)
+thm id\<^sub>T_cong[THEN rel_funD]
+term 0 (**)
+  
+lemma bind_cong[transfer_rule]:
+  fixes R0 R1
+  shows "(crel_ss R0 ===> (R0 ===> crel_ss R1) ===> crel_ss R1) (op \<bind>) (op \<bind>)"
+  unfolding rel_fun_def bind_def by (fastforce intro!: crel_ss_intro elim!: crel_ss_elim)
+thm bind_cong[THEN rel_funD, THEN rel_funD]
+term 0 (**)
+
+lemma app\<^sub>T_cong[transfer_rule]:
+  fixes R0 R1
+  shows "(crel_ss (R0 ===> crel_ss R1) ===> crel_ss R0 ===> crel_ss R1) (op .) (op .)"
+  unfolding fun_app_lifted_def by transfer_prover
+thm app\<^sub>T_cong[THEN rel_funD, THEN rel_funD]
+term 0 (**)
+
+lemma lift_33_cong[transfer_rule]:
+  fixes R0 R1 R2
+  shows "((R0 ===> R1 ===> R2) ===> crel_ss (R0 ===> crel_ss (R1 ===> crel_ss R2))) lift_33 lift_33"
+  unfolding lift_33_def by transfer_prover
+term 0 (**)
+    
+lemma Cons\<^sub>T_cong[transfer_rule]:
+  fixes R
+  shows "(crel_ss (R ===> crel_ss ((list_all2 R) ===> crel_ss (list_all2 R)))) Cons\<^sub>T Cons\<^sub>T"
+  unfolding Cons\<^sub>T_def by transfer_prover
+    
+term 0 (**)
+lemma map\<^sub>T_cong:
+  assumes "crel_ss (list_all2 R0) xs\<^sub>T ys\<^sub>T"
+  assumes "crel_ss (\<lambda>f g. crel_ss (list_all2 (\<lambda>x y. R0 x y \<longrightarrow> crel_ss R1 (f x) (g y))) xs\<^sub>T ys\<^sub>T) f\<^sub>T g\<^sub>T"
+  shows "crel_ss (list_all2 R1) (map\<^sub>T . f\<^sub>T . xs\<^sub>T) (map\<^sub>T . g\<^sub>T . ys\<^sub>T)"
+proof -
+  {
+    fix M assume "cmem M"
+    have map\<^sub>T': "runState map\<^sub>T M = (\<lambda>f. \<langle>map\<^sub>T' f\<rangle>, M)"
+      unfolding map\<^sub>T_def lift_3_def return_def by auto
+    obtain f Mf g Mg where
+      crel_xs_ys: "crel_ss (list_all2 (\<lambda>x y. R0 x y \<longrightarrow> crel_ss R1 (f x) (g y))) xs\<^sub>T ys\<^sub>T"
+      and f_g: "runState f\<^sub>T M = (f, Mf)" "runState g\<^sub>T M = (g, Mg)" "Mf = Mg" "cmem Mg"
+      using crel_ss_elim[OF assms(2) \<open>cmem M\<close>] .
+    obtain xs Mxs ys Mys where
+      crel_x_y: "list_all2 (\<lambda>x y. R0 x y \<longrightarrow> crel_ss R1 (f x) (g y)) xs ys"
+      and xs_ys: "runState xs\<^sub>T Mf = (xs, Mxs)" "runState ys\<^sub>T Mg = (ys, Mys)" "Mxs = Mys" "cmem Mys"
+      unfolding \<open>Mf = Mg\<close> using crel_ss_elim[OF crel_xs_ys \<open>cmem Mg\<close>] .
+    have "list_all2 R0 xs ys"
+      using assms(1) \<open>cmem Mg\<close> xs_ys \<open>Mf = Mg\<close> by (auto elim: crel_ss_elim)
+    with crel_x_y have "list_all2 (\<lambda>x y. crel_ss R1 (f x) (g y)) xs ys"
+      by (simp add: list_all2_conv_all_nth)
+    hence *:"crel_ss (list_all2 R1) (map\<^sub>T' f xs) (map\<^sub>T' g ys)"
+      proof (induction xs ys rule: list_all2_induct)
+        case Nil
+        then show ?case by (auto intro: crel_ss_intro simp: return_def)
+      next
+        case (Cons x xs y ys)
+        show ?case unfolding map\<^sub>T'.simps supply [transfer_rule]=Cons by transfer_prover
+      qed
+    obtain mxs Mmxs mys Mmys where
+      rel_mxs_mys: "list_all2 R1 mxs mys"
+      and mxs_mys: "runState (map\<^sub>T' f xs) Mxs = (mxs, Mmxs)"
+                   "runState (map\<^sub>T' g ys) Mys = (mys, Mmys)"
+                   "Mmxs = Mmys" "cmem Mmys"
+      unfolding \<open>Mxs = Mys\<close> using crel_ss_elim[OF * \<open>cmem Mys\<close>] .
+        
+    fix mxs' Mmxs' mys' Mmys'
+    assume "runState (map\<^sub>T . f\<^sub>T . xs\<^sub>T) M = (mxs', Mmxs')" "runState (map\<^sub>T . g\<^sub>T . ys\<^sub>T) M = (mys', Mmys')"
+    then have "mxs = mxs'" "mys = mys'" "Mmxs = Mmxs'" "Mmys = Mmys'"
+      unfolding
+        map\<^sub>T'[THEN fun_app_lifted_dest, OF f_g(1) runState_return, THEN fun_app_lifted_dest, OF xs_ys(1) mxs_mys(1)]
+        map\<^sub>T'[THEN fun_app_lifted_dest, OF f_g(2) runState_return, THEN fun_app_lifted_dest, OF xs_ys(2) mxs_mys(2)]
+      by auto
+    hence "list_all2 R1 mxs' mys' \<and> Mmxs' = Mmys' \<and> cmem Mmys'"
+      using rel_mxs_mys mxs_mys by auto
+  } from this[THEN crel_ss_intro] show ?thesis .
+qed
+
+end
+end
+end
