DP_Proof.thy
@@ -1,12 +1,12 @@
 theory DP_Proof
-  imports "./DP_Consistency" "~~/src/HOL/Eisbach/Eisbach_Tools"
+  imports "./DP_CRelVS" "~~/src/HOL/Eisbach/Eisbach_Tools"
 begin
 
 method dp_match uses induct simp simp\<^sub>T =
   ( rule dp_consistency.consistentDP_intro,
     induct_tac rule: induct,
     unfold simp\<^sub>T;
-    rule dp_consistency.consistentS_checkmem,
+    rule dp_consistency.crel_vs_checkmem,
     unfold simp,
     ((match premises in _[transfer_rule]: _ (multi) \<Rightarrow> transfer_prover)
       | (match conclusion in _ \<Rightarrow> transfer_prover)))
